Ensure hot code is inlined, add safety cond to unsafe bit shifts

SortingNetworkSearchFFI/c/extras.c
@@ -2,11 +2,11 @@
 #include <assert.h>
 
 uint64_t uShr64x8(uint64_t lhs, uint8_t rhs) {
-    assert(rhs <= 63 && "uShr64x8 rhs overflow");
+    assert(rhs <= 63 && "uShr64x8 attempt to right shift with overflow");
     return lhs >> rhs;
 }
 
 uint64_t uShl64x8(uint64_t lhs, uint8_t rhs) {
-    assert(rhs <= 63 && "uShl64x8 rhs overflow");
+    assert(rhs <= 63 && "uShl64x8 attempt to left shift with overflow");
     return lhs << rhs;
 }
